src/Solver/TD_Side_Soundness.thy
@@ -1,5 +1,5 @@
 theory TD_Side_Soundness
-  imports TD_Side_Interface Constraint_System_Sound
+  imports TD_Side_Interface Constraint_System_Sound Sign_Domain
 begin
 
 (*
@@ -15,7 +15,7 @@ begin
 
 theorem side_collect_sound_at_pp:
   fixes g :: cfg and tf :: "'a domain_transfer" and bot0 s0 :: "'a abs_state"
-    and S :: "store set" and v :: pp and x :: pp
+    and S :: "store set" and v :: pp
     and sigma :: "pp + unit => 'a abs_state" and vars :: "pp set"
   assumes tf_sound_assign:
     "\<forall>x a sg. \<forall>s \<in> gamma_state sg.
@@ -27,13 +27,12 @@ theorem side_collect_sound_at_pp:
     "\<forall>b sg. \<forall>s \<in> gamma_state sg. \<not> bval b s
        \<longrightarrow> s \<in> gamma_state (tf_assume_not tf b sg)"
   assumes fin_cfg: "finite (edges g)"
-  assumes pp: "part_post_solution (side_cfg_T g tf (\<squnion>) bot0 s0) x sigma vars"
-  assumes vars_reach: "\<And>u es w. g \<turnstile> u \<longrightarrow>\<^bsub>es\<^esub> w \<Longrightarrow> w \<in> vars"
+  assumes pp: "part_post_solution (side_cfg_T g tf (\<squnion>) bot0 s0) v sigma vars"
   assumes entry_cov: "S \<subseteq> gamma_state (side_env sigma (cfg_entry g))"
   assumes path: "g \<turnstile> (cfg_entry g) \<longrightarrow>\<^bsub>es\<^esub> v"
   shows "cfg_collect g S v \<le> gamma_state (side_env sigma v)"
   using side_collect_sound_at[OF tf_sound_assign tf_sound_assume tf_sound_assume_not
-    pp vars_reach fin_cfg entry_cov path] .
+    pp fin_cfg entry_cov path] .
 
 theorem side_analyse_collect_sound_at:
   fixes c :: com and tf :: "'a domain_transfer" and bot0 s0 :: "'a abs_state"
@@ -49,48 +48,43 @@ theorem side_analyse_collect_sound_at:
        \<longrightarrow> s \<in> gamma_state (tf_assume_not tf b sg)"
   assumes fin_cfg: "finite (edges (to_cfg c))"
   assumes pp:
-    "part_post_solution (side_cfg_T (to_cfg c) tf (\<squnion>) bot0 s0)
-       (cfg_entry (to_cfg c))
-       (td_cfg_side_solver.side_sigma_at (to_cfg c) tf bot0 s0 (cfg_entry (to_cfg c)))
-       (td_cfg_side_solver.side_stabl_at (to_cfg c) tf bot0 s0 (cfg_entry (to_cfg c)))"
+    "part_post_solution (side_cfg_T (to_cfg c) tf (\<squnion>) bot0 s0) v0
+       (td_cfg_side_solver.side_sigma_at (to_cfg c) tf bot0 s0 v0)
+       (td_cfg_side_solver.side_stabl_at (to_cfg c) tf bot0 s0 v0)"
   assumes entry_cov:
     "S \<subseteq> gamma_state
-       (side_env (td_cfg_side_solver.side_sigma_at (to_cfg c) tf bot0 s0 (cfg_entry (to_cfg c)))
+       (side_env (td_cfg_side_solver.side_sigma_at (to_cfg c) tf bot0 s0 v0)
                  (cfg_entry (to_cfg c)))"
-  assumes cfg_in_stabl:
-    "\<And>u es w. cfg_path (to_cfg c) u es w
-     \<Longrightarrow> w \<in> td_cfg_side_solver.side_stabl_at (to_cfg c) tf bot0 s0 (cfg_entry (to_cfg c))"
   assumes entry_path: "cfg_path (to_cfg c) (cfg_entry (to_cfg c)) es v0"
   shows "cfg_collect (to_cfg c) S v0
          \<le> gamma_state (side_analyse c tf bot0 s0 v0)"
 proof -
   define g where "g = to_cfg c"
-  define x where "x = cfg_entry g"
   define sigma where
-    "sigma = td_cfg_side_solver.side_sigma_at (to_cfg c) tf bot0 s0 (cfg_entry (to_cfg c))"
-  define vars where
-    "vars = td_cfg_side_solver.side_stabl_at (to_cfg c) tf bot0 s0 (cfg_entry (to_cfg c))"
+    "sigma = td_cfg_side_solver.side_sigma_at (to_cfg c) tf bot0 s0 v0"
   have g_def: "g = to_cfg c" by (simp add: g_def)
-  have x_def: "x = cfg_entry g" by (simp add: x_def g_def)
-  have sigma_def: "sigma = td_cfg_side_solver.side_sigma_at g tf bot0 s0 x"
-    by (simp add: sigma_def g_def x_def)
-  have vars_def: "vars = td_cfg_side_solver.side_stabl_at g tf bot0 s0 x"
-    by (simp add: vars_def g_def x_def)
-  have pp': "part_post_solution (side_cfg_T g tf (\<squnion>) bot0 s0) x sigma vars"
-    using pp unfolding g_def x_def sigma_def vars_def by simp
-  have vars_reach: "\<And>u es w. g \<turnstile> u \<longrightarrow>\<^bsub>es\<^esub> w \<Longrightarrow> w \<in> vars"
-    using cfg_in_stabl unfolding g_def x_def vars_def by auto
+  have sigma_def: "sigma = td_cfg_side_solver.side_sigma_at g tf bot0 s0 v0"
+    by (simp add: sigma_def g_def)
+  have pp': "part_post_solution (side_cfg_T g tf (\<squnion>) bot0 s0) v0 sigma
+             (td_cfg_side_solver.side_stabl_at g tf bot0 s0 v0)"
+    using pp unfolding g_def sigma_def by simp
   have entry: "S \<subseteq> gamma_state (side_env sigma (cfg_entry g))"
-    using entry_cov unfolding sigma_def g_def x_def by simp
-  have collect: "cfg_collect g S v0 \<le> gamma_state (side_env sigma v0)"
-    using side_collect_sound_at_pp[OF tf_sound_assign tf_sound_assume tf_sound_assume_not
-      fin_cfg[unfolded g_def] pp' vars_reach entry entry_path]
-    unfolding g_def .
-  show ?thesis
-    unfolding side_analyse_def td_cfg_side_solver.side_env_entry_def
-      td_cfg_side_solver.side_env_at_def side_env_def sigma_def g_def x_def
-    using collect by simp
+    using entry_cov unfolding sigma_def g_def by simp
+  have fin_g: "finite (edges g)" using fin_cfg unfolding g_def by simp
+  have path': "g \<turnstile> (cfg_entry g) \<longrightarrow>\<^bsub>es\<^esub> v0"
+    using entry_path unfolding g_def by simp
+  show "cfg_collect (to_cfg c) S v0 \<le> gamma_state (side_analyse c tf bot0 s0 v0)"
+  proof (rule order_trans)
+    show "cfg_collect (to_cfg c) S v0 \<le> gamma_state (side_env sigma v0)"
+      using side_collect_sound_at_pp[OF tf_sound_assign tf_sound_assume
+            tf_sound_assume_not fin_g pp' entry path']
+      unfolding g_def by simp
+    show "gamma_state (side_env sigma v0) \<le> gamma_state (side_analyse c tf bot0 s0 v0)"
+      unfolding side_analyse_def side_env_def sigma_def g_def
+      by (rule order_refl)
+  qed
 qed
+
 
 theorem side_analyse_collect_sound:
   fixes c :: com and tf :: "'a domain_transfer" and bot0 s0 :: "'a abs_state"
@@ -106,17 +100,13 @@ theorem side_analyse_collect_sound:
        \<longrightarrow> s \<in> gamma_state (tf_assume_not tf b sg)"
   assumes fin_cfg: "finite (edges (to_cfg c))"
   assumes pp:
-    "part_post_solution (side_cfg_T (to_cfg c) tf (\<squnion>) bot0 s0)
-       (cfg_entry (to_cfg c))
-       (td_cfg_side_solver.side_sigma_at (to_cfg c) tf bot0 s0 (cfg_entry (to_cfg c)))
-       (td_cfg_side_solver.side_stabl_at (to_cfg c) tf bot0 s0 (cfg_entry (to_cfg c)))"
+    "\<And>v. part_post_solution (side_cfg_T (to_cfg c) tf (\<squnion>) bot0 s0) v
+       (td_cfg_side_solver.side_sigma_at (to_cfg c) tf bot0 s0 v)
+       (td_cfg_side_solver.side_stabl_at (to_cfg c) tf bot0 s0 v)"
   assumes entry_cov:
-    "S \<subseteq> gamma_state
-       (side_env (td_cfg_side_solver.side_sigma_at (to_cfg c) tf bot0 s0 (cfg_entry (to_cfg c)))
+    "\<And>v. S \<subseteq> gamma_state
+       (side_env (td_cfg_side_solver.side_sigma_at (to_cfg c) tf bot0 s0 v)
                  (cfg_entry (to_cfg c)))"
-  assumes cfg_in_stabl:
-    "\<And>u es w. cfg_path (to_cfg c) u es w
-     \<Longrightarrow> w \<in> td_cfg_side_solver.side_stabl_at (to_cfg c) tf bot0 s0 (cfg_entry (to_cfg c))"
   assumes entry_reachable:
     "\<And>v. \<exists>es. cfg_path (to_cfg c) (cfg_entry (to_cfg c)) es v"
   shows "\<forall>v. cfg_collect (to_cfg c) S v
@@ -129,7 +119,7 @@ proof (intro allI)
   show "cfg_collect (to_cfg c) S v
         \<le> gamma_state (side_analyse c tf bot0 s0 v)"
     by (rule side_analyse_collect_sound_at[OF tf_sound_assign tf_sound_assume
-          tf_sound_assume_not fin_cfg pp entry_cov cfg_in_stabl entry_path])
+          tf_sound_assume_not fin_cfg pp entry_cov entry_path])
 qed
 
 theorem side_analyse_collect_sound_at_solver:
@@ -146,52 +136,178 @@ theorem side_analyse_collect_sound_at_solver:
        \<longrightarrow> s \<in> gamma_state (tf_assume_not tf b sg)"
   assumes tf_mono:
     "\<And>a s1 s2. s1 \<le> s2 \<Longrightarrow> apply_tf tf a s1 \<le> apply_tf tf a s2"
-  assumes fin_cfg: "finite (edges (to_cfg c))"
-  assumes entry_path: "cfg_path (to_cfg c) (cfg_entry (to_cfg c)) es v0"
-  assumes side_solve_dom: "side.solve_dom (cfg_entry (to_cfg c))"
+  assumes fin_cfg: "finite (edges (to_cfg c))"  assumes entry_path: "cfg_path (to_cfg c) (cfg_entry (to_cfg c)) es v0"
+  assumes side_solve_dom:
+    "side_cfg_solve_dom (to_cfg c) tf bot0 s0 v0"
   assumes S_sub: "S \<subseteq> gamma_state s0"
   assumes s0_global_bot: "restrict_global s0 = bot"
-  assumes cfg_in_stabl:
-    "\<And>u es w. cfg_path (to_cfg c) u es w
-     \<Longrightarrow> w \<in> td_cfg_side_solver.side_stabl_at (to_cfg c) tf bot0 s0 (cfg_entry (to_cfg c))"
   shows "cfg_collect (to_cfg c) S v0
          \<le> gamma_state (side_analyse c tf bot0 s0 v0)"
 proof -
-  interpret side: td_cfg_side_solver "to_cfg c" tf bot0 s0
+  interpret solver: td_cfg_side_solver "to_cfg c" tf bot0 s0
     using tf_mono by unfold_locales
-  have pp: "part_post_solution side.cfg_side_T (cfg_entry (to_cfg c))
-             (side.side_sigma_at (cfg_entry (to_cfg c)))
-             (side.side_stabl_at (cfg_entry (to_cfg c)))"
-    using side.side_solver_part_post_at_entry[OF side_solve_dom] by simp
+  have pp: "part_post_solution solver.cfg_side_T v0 (solver.side_sigma_at v0) (solver.side_stabl_at v0)"
+    using solver.side_solver_part_post_at_cfg[OF side_solve_dom] by simp
+  define g where "g = to_cfg c"
+  have g_def: "g = to_cfg c" by (simp add: g_def)
+  have pp': "part_post_solution (side_cfg_T g tf (\<squnion>) bot0 s0) v0
+             (solver.side_sigma_at v0) (solver.side_stabl_at v0)"
+    using pp unfolding g_def solver.cfg_side_T_eq by simp
+  have fin: "finite (edges g)" using fin_cfg unfolding g_def by simp
+  have entry_path': "g \<turnstile> cfg_entry g \<longrightarrow>\<^bsub>es\<^esub> v0"
+    using entry_path unfolding g_def by simp
+  have entry_in: "cfg_entry g \<in> solver.side_stabl_at v0"
+    using side_vars_on_query_path[OF pp' fin entry_path'] by simp
   have entry_cov: "S \<subseteq> gamma_state
-       (side_env (side.side_sigma_at (cfg_entry (to_cfg c))) (cfg_entry (to_cfg c)))"
+       (side_env (solver.side_sigma_at v0) (cfg_entry g))"
   proof -
-    have acc0_le: "bot0 \<squnion> restrict_local s0
-                   \<le> side.side_sigma_at (cfg_entry (to_cfg c)) (Inl (cfg_entry (to_cfg c)))"
-      using side_post_solution_le_local[OF pp side.side_entry_in_stabl[OF side_solve_dom]]
-      unfolding eq_side_cfg_T side.cfg_side_T_def by simp
+    have local_le: "side_acc tf (\<squnion>) (bot0 \<squnion> restrict_local s0) (solver.side_sigma_at v0)
+                     (predecessor_list g (cfg_entry g))
+                   \<le> solver.side_sigma_at v0 (Inl (cfg_entry g))"
+      using side_post_solution_le_local[OF pp' entry_in] unfolding g_def by simp
+    have acc0_le: "bot0 \<squnion> restrict_local s0 \<le> solver.side_sigma_at v0 (Inl (cfg_entry g))"
+      using side_acc_ge_acc local_le by (rule order_trans)
     have s0_le: "s0 \<le> bot0 \<squnion> restrict_local s0"
     proof (rule le_funI)
       fix x
       show "s0 x \<le> (bot0 \<squnion> restrict_local s0) x"
       proof (cases "is_global x")
         case True
-        then show ?thesis using s0_global_bot unfolding restrict_global_def by simp
+        have "restrict_global s0 x = bot x"
+          using s0_global_bot by (simp add: fun_eq_iff restrict_global_def)
+        then show ?thesis using True unfolding restrict_global_def by simp
       next
         case False
         then show ?thesis unfolding restrict_local_def using sup_ge2 by simp
       qed
     qed
-    have "s0 \<le> side_env (side.side_sigma_at (cfg_entry (to_cfg c))) (cfg_entry (to_cfg c))"
-      unfolding side_env_def using acc0_le s0_le sup_ge1 sup_left_mono by auto
+    have sigma_le: "s0 \<le> solver.side_sigma_at v0 (Inl (cfg_entry g))"
+      using acc0_le s0_le by (auto intro: order_trans)
+    have "s0 \<le> side_env (solver.side_sigma_at v0) (cfg_entry g)"
+      unfolding side_env_def by (rule order_trans[OF sigma_le sup_ge1])
     thus ?thesis using S_sub gamma_state_mono by blast
   qed
   show ?thesis
-    using side_analyse_collect_sound_at[OF tf_sound_assign tf_sound_assume
-      tf_sound_assume_not fin_cfg pp entry_cov cfg_in_stabl entry_path]
-    by simp
+  proof (rule side_analyse_collect_sound_at)
+    show "part_post_solution (side_cfg_T (to_cfg c) tf (\<squnion>) bot0 s0) v0
+          (td_cfg_side_solver.side_sigma_at (to_cfg c) tf bot0 s0 v0)
+          (td_cfg_side_solver.side_stabl_at (to_cfg c) tf bot0 s0 v0)"
+      using pp' unfolding g_def by simp
+    show "S \<subseteq> gamma_state
+          (side_env (td_cfg_side_solver.side_sigma_at (to_cfg c) tf bot0 s0 v0)
+                    (cfg_entry (to_cfg c)))"
+      using entry_cov unfolding g_def by simp
+    show "\<forall>x a sg. \<forall>s \<in> gamma_state sg. s(x := aval a s) \<in> gamma_state (tf_assign tf x a sg)"
+      using tf_sound_assign .
+    show "\<forall>b sg. \<forall>s \<in> gamma_state sg. bval b s \<longrightarrow> s \<in> gamma_state (tf_assume tf b sg)"
+      using tf_sound_assume .
+    show "\<forall>b sg. \<forall>s \<in> gamma_state sg. \<not> bval b s \<longrightarrow> s \<in> gamma_state (tf_assume_not tf b sg)"
+      using tf_sound_assume_not .
+    show "finite (edges (to_cfg c))" using fin_cfg .
+    show "cfg_path (to_cfg c) (cfg_entry (to_cfg c)) es v0" using entry_path .
+  qed
+qed
+
+theorem side_analyse_collect_sound_solver:
+  fixes c :: com and tf :: "'a domain_transfer" and bot0 s0 :: "'a abs_state"
+    and S :: "store set"
+  assumes tf_sound_assign:
+    "\<forall>x a sg. \<forall>s \<in> gamma_state sg.
+       s(x := aval a s) \<in> gamma_state (tf_assign tf x a sg)"
+  assumes tf_sound_assume:
+    "\<forall>b sg. \<forall>s \<in> gamma_state sg. bval b s
+       \<longrightarrow> s \<in> gamma_state (tf_assume tf b sg)"
+  assumes tf_sound_assume_not:
+    "\<forall>b sg. \<forall>s \<in> gamma_state sg. \<not> bval b s
+       \<longrightarrow> s \<in> gamma_state (tf_assume_not tf b sg)"
+  assumes tf_mono:
+    "\<And>a s1 s2. s1 \<le> s2 \<Longrightarrow> apply_tf tf a s1 \<le> apply_tf tf a s2"
+  assumes fin_cfg: "finite (edges (to_cfg c))"
+  assumes entry_reachable:
+    "\<And>v. \<exists>es. cfg_path (to_cfg c) (cfg_entry (to_cfg c)) es v"
+  assumes side_solve_dom:
+    "\<And>v. side_cfg_solve_dom (to_cfg c) tf bot0 s0 v"
+  assumes S_sub: "S \<subseteq> gamma_state s0"
+  assumes s0_global_bot: "restrict_global s0 = bot"
+  shows "\<forall>v. cfg_collect (to_cfg c) S v
+         \<le> gamma_state (side_analyse c tf bot0 s0 v)"
+proof (intro allI)
+  fix v
+  obtain es where entry_path:
+    "cfg_path (to_cfg c) (cfg_entry (to_cfg c)) es v"
+    using entry_reachable by blast
+  show "cfg_collect (to_cfg c) S v
+        \<le> gamma_state (side_analyse c tf bot0 s0 v)"
+    by (rule side_analyse_collect_sound_at_solver[OF tf_sound_assign tf_sound_assume
+          tf_sound_assume_not tf_mono fin_cfg entry_path side_solve_dom S_sub
+          s0_global_bot])
+qed
+
+theorem side_solver_sound:
+  fixes c :: com and tf :: "'a domain_transfer" and bot0 s0 :: "'a abs_state"
+    and s t :: store and es :: "(edge_action * pp) list"
+  assumes tf_sound_assign:
+    "\<forall>x a sg. \<forall>s \<in> gamma_state sg.
+       s(x := aval a s) \<in> gamma_state (tf_assign tf x a sg)"
+  assumes tf_sound_assume:
+    "\<forall>b sg. \<forall>s \<in> gamma_state sg. bval b s
+       \<longrightarrow> s \<in> gamma_state (tf_assume tf b sg)"
+  assumes tf_sound_assume_not:
+    "\<forall>b sg. \<forall>s \<in> gamma_state sg. \<not> bval b s
+       \<longrightarrow> s \<in> gamma_state (tf_assume_not tf b sg)"
+  assumes tf_mono:
+    "\<And>a s1 s2. s1 \<le> s2 \<Longrightarrow> apply_tf tf a s1 \<le> apply_tf tf a s2"
+  assumes s0_sound: "s \<in> gamma_state s0"
+  assumes exit_in_collect:
+    "t \<in> cfg_collect (to_cfg c) {s} (cfg_exit (to_cfg c))"
+  assumes fin_cfg: "finite (edges (to_cfg c))"
+  assumes entry_path:
+    "cfg_path (to_cfg c) (cfg_entry (to_cfg c)) es (cfg_exit (to_cfg c))"
+  assumes side_solve_dom:
+    "side_cfg_solve_dom (to_cfg c) tf bot0 s0 (cfg_exit (to_cfg c))"
+  assumes s0_global_bot: "restrict_global s0 = bot"
+  shows "t \<in> gamma_state (side_analyse c tf bot0 s0 (cfg_exit (to_cfg c)))"
+proof -
+  have S_sub: "{s} \<subseteq> gamma_state s0" using s0_sound by auto
+  have collect: "cfg_collect (to_cfg c) {s} (cfg_exit (to_cfg c))
+    \<le> gamma_state (side_analyse c tf bot0 s0 (cfg_exit (to_cfg c)))"
+    by (rule side_analyse_collect_sound_at_solver[OF tf_sound_assign tf_sound_assume
+          tf_sound_assume_not tf_mono fin_cfg entry_path side_solve_dom S_sub
+          s0_global_bot])
+  show ?thesis using collect exit_in_collect by blast
 qed
 
 end
+
+(* -- Sign Domain Instantiation ----------------------------------- *)
+
+theorem side_sign_analysis_sound:
+  fixes c :: com and s t :: store and es :: "(edge_action * pp) list"
+  assumes s_sound: "s \<in> sign_domain.gamma_state s0"
+  assumes exit_in_collect:
+    "t \<in> cfg_collect (to_cfg c) {s} (cfg_exit (to_cfg c))"
+  assumes fin_cfg: "finite (edges (to_cfg c))"
+  assumes entry_path:
+    "cfg_path (to_cfg c) (cfg_entry (to_cfg c)) es (cfg_exit (to_cfg c))"
+  assumes side_solve_dom:
+    "side_cfg_solve_dom (to_cfg c) sign_tf bot s0 (cfg_exit (to_cfg c))"
+  assumes s0_global_bot: "restrict_global s0 = bot"
+  shows "t \<in> sign_domain.gamma_state
+       (side_analyse c sign_tf bot s0 (cfg_exit (to_cfg c)))"
+proof -
+  have h1: "\<forall>x a sigma. \<forall>s \<in> sign_domain.gamma_state sigma.
+              s(x := aval a s) \<in> sign_domain.gamma_state (tf_assign sign_tf x a sigma)"
+    unfolding sign_tf_def by (simp add: assign_sign_sound)
+  have h2: "\<forall>b sigma. \<forall>s \<in> sign_domain.gamma_state sigma.
+              bval b s \<longrightarrow> s \<in> sign_domain.gamma_state (tf_assume sign_tf b sigma)"
+    unfolding sign_tf_def by (simp add: assume_sign_sound)
+  have h3: "\<forall>b sigma. \<forall>s \<in> sign_domain.gamma_state sigma.
+              \<not> bval b s \<longrightarrow> s \<in> sign_domain.gamma_state (tf_assume_not sign_tf b sigma)"
+    unfolding sign_tf_def by (simp add: assume_not_sign_sound)
+  show ?thesis
+    by (rule sign_domain.side_solver_sound
+          [OF h1 h2 h3 sign_tf_mono s_sound exit_in_collect fin_cfg entry_path
+            side_solve_dom s0_global_bot])
+qed
 
 end
